add some commments

code/ReifyNExpr.v
@@ -1,3 +1,4 @@
+(* Note from Dan: my comments in the code are prefixed with `DF'. *)
 Require Import Coq.Strings.String.
 Require Import MetaCoq.Template.All.
 Require Import Switch.Switch.
@@ -19,9 +20,17 @@ Run TemplateProgram (mkSwitch string
                                  ("Coq.Init.Nat.mul", "n_Mul")]
                               "NOp_Names" "parse_NOp_Name").
 
+(* DF: to see what did the previous command do:
+Print NOp_Names.
+Check parse_NOp_Name.
+Eval compute in (parse_NOp_Name "Coq.Init.Nat.add"). *)
+
 Definition inat :=  {| inductive_mind := "Coq.Init.Datatypes.nat";
                        inductive_ind := 0 |}.
 Definition nt := tInd inat [].
+(* DF:
+Check inat.
+Check nt. *)
 Definition ilist := {| inductive_mind := "Coq.Init.Datatypes.list";
                        inductive_ind := 0 |}.
 
@@ -29,7 +38,9 @@ Definition varlist:Type := list string.
 
 Fixpoint compileNExpr (params:varlist) (a_n:term): TemplateMonad (varlist*NExpr) :=
   match a_n with
+  (* Case 0 *)
   | tConstruct inat 0 [] => tmReturn (params, NConst 0)
+  (* Case (S e) *)
   | tApp (tConstruct inat 1 []) [e] =>
     d_e <- compileNExpr params e ;;
         let '(_, d_e') := d_e in
@@ -37,27 +48,44 @@ Fixpoint compileNExpr (params:varlist) (a_n:term): TemplateMonad (varlist*NExpr)
                            | NConst v => NConst (S v)
                            | o => NPlus o (NConst 1)
                            end))
+  (* Case binary function f (a_a, a_b) *)
   | tApp (tConst bfun []) [ a_a ; a_b] =>
     d_a <- compileNExpr params a_a ;;
-        d_b <- compileNExpr params a_b ;;
-        let '(_, d_a') := d_a in
-        let '(_, d_b') := d_b in
-        match parse_NOp_Name bfun with
-        | Some n_Add => tmReturn (params, NPlus  d_a' d_b')
-        | Some n_Sub => tmReturn (params, NMinus d_a' d_b')
-        | Some n_Mul => tmReturn (params, NMult  d_a' d_b')
-        | None => tmFail ("Unknown binary function" ++ bfun)
-        end
+    d_b <- compileNExpr params a_b ;;
+    let '(_, d_a') := d_a in
+    let '(_, d_b') := d_b in
+    match parse_NOp_Name bfun with
+    | Some n_Add => tmReturn (params, NPlus  d_a' d_b')
+    | Some n_Sub => tmReturn (params, NMinus d_a' d_b')
+    | Some n_Mul => tmReturn (params, NMult  d_a' d_b')
+    | None => tmFail ("Unknown binary function" ++ bfun)
+    end
+  (* The last two cases are for dealing with variables *)
   | tLambda (nNamed n) nt b_n =>  compileNExpr (n::params) b_n
   | tRel n => tmReturn (params, NVar n)
   | _ => tmFail ("Unsupported NExpr" ++ (string_of_term a_n))
   end.
 
+(* DF: using compileNExpr :
+Definition test_compileNExpr (t : term) : TemplateMonad unit :=
+  r <- compileNExpr [] t ;;
+  let '(params, res) := r in
+  nres <- tmEval all res ;;
+  tmPrint params ;;
+  tmPrint res ;;
+  tmPrint nres.
+
+Quote Definition test1 := (1 + 0).
+Quote Definition test2 := (fun x => x * (0 + 1)).
+Run TemplateProgram ( test_compileNExpr test1 ).
+Run TemplateProgram ( test_compileNExpr test2 ).
+*)
+
 Fixpoint build_param_list (l:varlist) : TemplateMonad term :=
   match l with
   | [] => tmReturn (tApp (tConstruct ilist 0 []) [nt])
   | x::xs => ts <- build_param_list xs ;;
-               tmReturn (tApp (tConstruct ilist 1 []) [nt; tRel (length xs); ts])
+             tmReturn (tApp (tConstruct ilist 1 []) [nt; tRel (length xs); ts])
   end.
 
 Definition build_forall (p:varlist) conc :=
@@ -83,9 +111,31 @@ Polymorphic Definition reifyNExp {A:Type}
   let lemma_concl := tApp (tConst "NExpr_term_equiv" []) [a_params; a_c; a_exp] in
   let lemma_ast := build_forall params lemma_concl in
   (tmBind (tmUnquoteTyped Prop lemma_ast)
-          (fun lemma_body => tmLemma lemma_name lemma_body
-                             ;;
+          (fun lemma_body => _ <- tmLemma lemma_name lemma_body ;;
                              tmReturn tt)).
+
+(* DF: example usage
+Run TemplateProgram (reifyNExp "e1" "e1_correct" (2 + 1 * 0)).
+Next Obligation. vm_compute; reflexivity. Qed.
+Print e1.
+Check e1_correct.
+*)
+
+(* DF: This is a more complicated example, where we cannot just solve
+the goal by `reflexivity':
+
+Run TemplateProgram (reifyNExp "e2" "e2_correct" (fun (x : nat) => 2 + x)).
+Next Obligation.
+  unfold NExpr_term_equiv. simpl.
+  rewrite <- plus_n_Sm.
+  rewrite <- plus_n_Sm.
+  rewrite <- (plus_n_O x).
+  rewrite <- (plus_n_O (S x)).
+  reflexivity.
+Qed.
+Print e2.
+Check e2_correct.
+*)
 
 (* -- Proof automation  -- *)
 
@@ -149,3 +199,6 @@ Run TemplateProgram (reifyNExp "Ex1_def" "Ex1_lemma" Ex1).
 
 Print Ex1_def.
 Check Ex1_lemma.
+
+(* DF: as an exercise, what would be needed to implement
+      things like let binding in this embedded language? *)
